src/ShouldBuild.v
@@ -24,8 +24,8 @@ From Perennial.program_proof Require
      wp_to_wpc.
 From Perennial.program_proof.examples Require
      all_examples.
-From Perennial.program_proof.lockservice Require
-     rpc bank_proof kv_durable incr_proof incr_proxy_proof.
+(* From Perennial.program_proof.lockservice Require
+     rpc bank_proof kv_durable incr_proof incr_proxy_proof. *)
 From Perennial.goose_lang Require
      ffi.append_log_ffi
      ffi.kvs_ffi.
